Work out another compatibility lemma. Redefine observation to require observation of termination to take at least one step, making some things more convenient. There's some duplication in the definitions of TerminatingN and Observe that we should probably factor out somehow.

LogRel/LR.v
@@ -48,10 +48,17 @@ Definition lev : World → nat := fun w => w.
 Definition PTRel := PTy -> S.Tm -> U.UTm -> Prop.
 Definition PCRel := PTy -> S.PCtx -> U.PCtx -> Prop.
 
+(* Intuitively: observing termination takes a step in addition to the actual evaluation steps *)
+Definition Observe (n : nat) (T : nat -> Prop) : Prop :=
+  match n with 
+      | 0 => False
+      | S n' => T n'
+  end.
+
 Definition Obs (d : Direction) (w : World) (ts : S.Tm) (tu : U.UTm) :=
   match d with
-    | dir_lt => S.TerminatingN ts (lev w) → U.Terminating tu
-    | dir_gt => U.TerminatingN tu (lev w) → S.Terminating ts
+    | dir_lt => Observe (lev w) (S.TerminatingN ts) → U.Terminating tu
+    | dir_gt => Observe (lev w) (U.TerminatingN tu)  → S.Terminating ts
   end.
 
 Definition contrel'
